checkpoint of SSA p&p.
git-svn-id: https://webdav.seas.upenn.edu/svn/sol/vol@2938 eef5ea85-cc2e-0410-bd84-0fae1f012da8

src/ssa/ssa_wf.v
@@ -23,8 +23,768 @@ Require Import Iteration.
 Require Import Kildall.
 Require Import ssa_analysis.
 Require Import ssa_static.
+Require Import ssa_dynamic.
 
 Export LLVMwf.
+
+  Definition getCmdID' (i:cmd) : option id :=
+  match i with
+  | insn_bop id _ sz v1 v2 => Some id
+  | insn_fbop id _ _ _ _ => Some id
+  (* | insn_extractelement id typ0 id0 c1 => id *)
+  (* | insn_insertelement id typ0 id0 typ1 v1 c2 => id *)
+  | insn_extractvalue id typs id0 c1 => Some id
+  | insn_insertvalue id typs id0 typ1 v1 c2 => Some id 
+  | insn_malloc id _ _ _ => Some id
+  | insn_free id _ _ => None
+  | insn_alloca id _ _ _ => Some id
+  | insn_load id typ1 v1 _ => Some id
+  | insn_store id typ1 v1 v2 _ => None
+  | insn_gep id _ _ _ _ => Some id
+  | insn_trunc id _ typ1 v1 typ2 => Some id 
+  | insn_ext id _ sz1 v1 sz2 => Some id
+  | insn_cast id _ typ1 v1 typ2 => Some id
+  | insn_icmp id cond typ v1 v2 => Some id
+  | insn_fcmp id cond typ v1 v2 => Some id 
+  | insn_select id v0 typ v1 v2 => Some id
+  | insn_call id nr _ typ v0 paraml => if nr then None else Some id
+  end.
+ 
+Fixpoint cmds_dominates_cmd_aux (cs:cmds) (id0:id) (ctx:atoms) : option atoms :=
+match cs with
+| nil => None
+| c1::cs' => 
+    match getCmdID' c1 with
+    | Some id1 =>
+      if eq_atom_dec id1 id0 then 
+        Some ctx 
+      else cmds_dominates_cmd_aux cs' id0 ({{id1}} `union` ctx)
+    | None => Some ctx
+    end
+end.
+
+Definition cmds_dominates_cmd (cs:cmds) (id0:id) : option atoms :=
+cmds_dominates_cmd_aux cs id0 {}. 
+
+Fixpoint getCmdsIDs (cs:cmds) : atoms :=
+match cs with
+| nil => {}
+| c::cs' =>
+    match getCmdID' c with 
+    | Some id1 => {{id1}} `union` getCmdsIDs cs'
+    | None => getCmdsIDs cs'
+    end
+end.
+
+Fixpoint getPhiNodesIDs' (ps: phinodes) : atoms :=
+match ps with
+| nil => {}
+| p::ps' => 
+    let id1 := getPhiNodeID p in 
+    {{id1}} `union` getPhiNodesIDs' ps'
+end.
+
+Definition getBlockIDs (b:block) : atoms :=
+let '(block_intro _ ps cs _) := b in
+getPhiNodesIDs' ps `union` getCmdsIDs cs.
+
+Fixpoint getArgsIDs (la:args) : atoms :=
+match la with
+| nil => {}
+| (_,id1)::la' => {{id1}} `union` getArgsIDs la'
+end.
+
+Definition inscope_of_cmd (f:fdef) (b1:block) (c:cmd) : option atoms :=
+let id0 := getCmdID c in
+let '(block_intro l1 ps cs _) := b1 in
+let '(fdef_intro (fheader_intro _ _ la) _) := f in
+let 'dt := dom_analyze f in
+let '(Dominators.mkBoundedSet els _) := AMap.get l1 dt in
+match cmds_dominates_cmd cs id0 with
+| None => None
+| Some ids' => 
+    fold_left 
+      (fun (opt_ctx:option atoms) (lbl:l) =>
+         match opt_ctx with
+         | Some ctx =>
+           match lookupBlockViaIDFromFdef f lbl with
+           | None => None
+           | Some b => 
+               if eq_atom_dec lbl l1 then Some ctx
+               else Some (getBlockIDs b `union` ctx)
+           end
+         | None => None
+         end
+      )
+      (AtomSetImpl.elements els) 
+      (Some (getPhiNodesIDs' ps `union` ids' `union` getArgsIDs la))
+end.
+
+Definition inscope_of_tmn (f:fdef) (b1:block) (tmn:terminator) : option atoms :=
+let '(block_intro l1 ps cs _) := b1 in
+let '(fdef_intro (fheader_intro _ _ la) _) := f in
+let 'dt := dom_analyze f in
+let '(Dominators.mkBoundedSet els _) := AMap.get l1 dt in
+fold_left 
+  (fun (opt_ctx:option atoms) (lbl:l) =>
+     match opt_ctx with
+     | Some ctx =>
+       match lookupBlockViaIDFromFdef f lbl with
+       | None => None
+       | Some b => 
+         if eq_atom_dec lbl l1 then Some ctx
+         else Some (getBlockIDs b `union` ctx)
+       end
+     | None => None
+     end
+  )
+  (AtomSetImpl.elements els) 
+  (Some (getPhiNodesIDs' ps `union` getCmdsIDs cs `union` getArgsIDs la)).
+
+Definition defs_dominate (f:fdef) (curb incomingb:block) (i:insn) : option atoms 
+  :=
+match i with
+| insn_phinode p => 
+    let '(block_intro _ _ _ tmn) := incomingb in
+    inscope_of_tmn f incomingb tmn
+| insn_cmd c => inscope_of_cmd f curb c
+| insn_terminator tmn => inscope_of_tmn f curb tmn
+end.
+
+Export LLVMgv.
+Export LLVMopsem.
+
+(* FIXME: this could be the tricky part. *)
+Inductive wf_genericvalue : GenericValue -> typ -> Prop :=
+| wf_genericvalue_intro : forall gv t, wf_genericvalue gv t.
+
+Inductive wf_defs : fdef -> GVMap -> ids -> Prop :=
+| wf_defs_nil : forall f lc, wf_defs f lc nil
+| wf_defs_cons : forall f lc id1 gv1 t1 ids',
+    lookupTypViaIDFromFdef f id1 = Some t1 ->
+    wf_genericvalue gv1 t1 ->
+    wf_defs f lc ids' ->
+    wf_defs f lc (id1::ids')
+.
+
+Definition wf_ExecutionContext (ps:list product) (ec:ExecutionContext) : Prop :=
+let '(mkEC f b cs tmn lc als) := ec in
+blockInFdefB b f = true /\
+InProductsB (product_fdef f) ps = true /\
+match cs with
+| nil => 
+    match inscope_of_tmn f b tmn with
+    | Some ids => wf_defs f lc (AtomSetImpl.elements ids)
+    | None => False
+    end
+| c::_ =>
+    match inscope_of_cmd f b c with
+    | Some ids => wf_defs f lc (AtomSetImpl.elements ids)
+    | None => False
+    end
+end /\
+exists l1, exists ps, exists cs',
+b = block_intro l1 ps (cs'++cs) tmn.
+
+Definition wf_call (ec:ExecutionContext) (ecs:ECStack) : Prop :=
+let '(mkEC f b cs tmn lc als) := ec in
+match tmn with
+| insn_return _ _ _ =>
+    match ecs with
+    | nil => True
+    | mkEC f' b' (insn_call _ _ _ _ _ _ ::_) tmn' lc' als'::ecs' => True
+    | _ => False
+    end
+| insn_return_void _ =>
+    match ecs with
+    | nil => True
+    | mkEC f' b' (insn_call _ true _ _ _ _ ::_) tmn' lc' als'::ecs' => True
+    | _ => False
+    end
+| _ => True
+end.
+
+Fixpoint wf_ECStack (ps:list product) (ecs:ECStack) : Prop :=
+match ecs with
+| nil => True
+| ec::ecs' => wf_ExecutionContext ps ec /\ wf_ECStack ps ecs' /\ wf_call ec ecs'
+end.
+
+Definition wf_State (S:State) : Prop :=
+let '(mkState s (los, nts) ps ecs _ _ _) := S in
+wf_system nil s /\
+moduleInSystemB (module_intro los nts ps) s = true /\
+wf_ECStack ps ecs.
+
+Lemma inscope_of_cmd_tmn : forall f l2 ps2 cs2' c' tmn' ids1,
+Some ids1 = inscope_of_cmd f (block_intro l2 ps2 (cs2'++[c']) tmn') c' ->
+exists ids2, 
+  Some ids2 = inscope_of_tmn f (block_intro l2 ps2 (cs2'++[c']) tmn') tmn' /\
+  match getCmdID' c' with
+  | Some id1 => {{id1}} `union` ids1 [=] ids2
+  | None => ids1 [=] ids2
+  end.
+Admitted.
+
+Lemma wf_defs_updateAddAL : forall g TD Mem' Result lc gl F' lc' t ids2 i1,
+  ret g = getOperandValue TD Mem' Result lc gl ->
+  wf_defs F' lc' (AtomSetImpl.elements t) ->
+  union (singleton i1) t[=]ids2 ->
+  wf_defs F' (updateAddAL GenericValue lc' i1 g) (AtomSetImpl.elements ids2).
+Admitted.
+
+Lemma wf_defs_eq : forall ids1 ids2 F' lc',
+  ids1 [=] ids2 ->
+  wf_defs F' lc' (AtomSetImpl.elements ids1) ->
+  wf_defs F' lc' (AtomSetImpl.elements ids2).
+Admitted.
+
+Lemma inscope_of_cmd_cmd : forall f l2 ps2 cs2' c' c cs' tmn' ids1,
+Some ids1 = inscope_of_cmd f (block_intro l2 ps2 (cs2'++[c']++[c]++cs') tmn') c' 
+  ->
+exists ids2, 
+  Some ids2 = 
+    inscope_of_cmd f (block_intro l2 ps2 (cs2'++[c']++[c]++cs') tmn') c /\
+  match getCmdID' c' with
+  | Some id1 => {{id1}} `union` ids1 [=] ids2
+  | None => ids1 [=] ids2
+  end.
+Admitted.
+
+Lemma inscope_of_tmn_br : forall F l0 ps cs bid l1 l2 ids0 l' ps' cs' tmn' Cond 
+  c TD Mem0 gl lc,
+Some ids0 = inscope_of_tmn F (block_intro l0 ps cs (insn_br bid Cond l1 l2)) 
+  (insn_br bid Cond l1 l2) ->
+getOperandValue TD Mem0 Cond lc gl = ret c ->
+Some (block_intro l' ps' cs' tmn') =
+       (if isGVZero TD c
+        then lookupBlockViaLabelFromFdef F l2
+        else lookupBlockViaLabelFromFdef F l1) ->
+exists ids0',
+  match cs' with
+  | nil => Some ids0' = inscope_of_tmn F (block_intro l' ps' cs' tmn') tmn'
+  | c'::_ => Some ids0' = inscope_of_cmd F (block_intro l' ps' cs' tmn') c'
+  end /\
+  AtomSetImpl.diff ids0' (getPhiNodesIDs' ps') [<=] ids0.
+Admitted.
+
+Lemma wf_defs_br : forall TD Mem0 Cond lc gl c l' ps' cs' lc' F l1 l2 bid tmn'
+  (H : getOperandValue TD Mem0 Cond lc gl = ret c)
+  (H0 : ret block_intro l' ps' cs' tmn' =
+       (if isGVZero TD c
+        then lookupBlockViaLabelFromFdef F l2
+        else lookupBlockViaLabelFromFdef F l1))
+  (l3 : l)
+  (ps3 : phinodes)
+  (cs3' : list cmd)
+  (H1 : switchToNewBasicBlock TD Mem0 (block_intro l' ps' cs' tmn')
+         (block_intro l3 ps3 (cs3' ++ nil) (insn_br bid Cond l1 l2)) gl lc =
+       ret lc')
+  (t : atoms)
+  (Hinscope1 : wf_defs F lc (AtomSetImpl.elements t))
+  (ids0' : atoms)
+  (HeqR12 : AtomSetImpl.diff ids0' (getPhiNodesIDs' ps')[<=]t),
+  wf_defs F lc' (AtomSetImpl.elements ids0').
+Admitted.
+
+Lemma inscope_of_tmn_br_uncond : forall F l3 ps cs bid ids0 l' ps' cs' tmn' l0,
+Some ids0 = inscope_of_tmn F (block_intro l3 ps cs (insn_br_uncond bid l0)) 
+  (insn_br_uncond bid l0) ->
+Some (block_intro l' ps' cs' tmn') = lookupBlockViaLabelFromFdef F l0 ->
+exists ids0',
+  match cs' with
+  | nil => Some ids0' = inscope_of_tmn F (block_intro l' ps' cs' tmn') tmn'
+  | c'::_ => Some ids0' = inscope_of_cmd F (block_intro l' ps' cs' tmn') c'
+  end /\
+  AtomSetImpl.diff ids0' (getPhiNodesIDs' ps') [<=] ids0.
+Admitted.
+
+Lemma wf_defs_br_uncond : forall lc l' ps' cs' lc' F bid tmn' gl l0 TD 
+  Mem0
+  (H0 : ret block_intro l' ps' cs' tmn' =lookupBlockViaLabelFromFdef F l0)
+  (l3 : l)
+  (ps3 : phinodes)
+  (cs3' : list cmd)
+  (H1 : switchToNewBasicBlock TD Mem0 (block_intro l' ps' cs' tmn')
+         (block_intro l3 ps3 (cs3' ++ nil) (insn_br_uncond bid l0)) gl lc =
+       ret lc')
+  (t : atoms)
+  (Hinscope1 : wf_defs F lc (AtomSetImpl.elements t))
+  (ids0' : atoms)
+  (HeqR12 : AtomSetImpl.diff ids0' (getPhiNodesIDs' ps')[<=]t),
+  wf_defs F lc' (AtomSetImpl.elements ids0').
+Admitted.
+
+
+Lemma wf_system__wf_insn : forall l1 ps1 cs1 tmn1 f ps los nts s ifs,
+  blockInFdefB (block_intro l1 ps1 cs1 tmn1) f = true -> 
+  InProductsB (product_fdef f) ps = true ->
+  moduleInSystemB (module_intro los nts ps) s = true ->
+  wf_system ifs s ->
+  wf_insn ifs s (module_intro los nts ps) f (block_intro l1 ps1 cs1 tmn1) 
+    (insn_terminator tmn1).
+Admitted.
+
+Lemma preservation : forall S1 S2 tr,
+  dsInsn S1 S2 tr -> wf_State S1 -> wf_State S2.
+Proof.
+  intros S1 S2 tr HdsInsn HwfS1.
+  (dsInsn_cases (induction HdsInsn) Case); destruct TD as [los nts].
+Focus.
+Case "dsReturn".
+  destruct HwfS1 as 
+    [HwfSystem [HmInS [
+     [HBinF1 [HFinPs1 [Hinscope1 [l1 [ps1 [cs1' Heq1]]]]]] 
+     [
+       [
+         [HBinF2 [HFinPs2 [Hinscope2 [l2 [ps2 [cs2' Heq2]]]]]] 
+         [HwfEC HwfCall]
+       ]
+       HwfCall'
+     ]
+    ]]]; subst.
+  remember (inscope_of_cmd F' (block_intro l2 ps2 (cs2' ++ c' :: cs') tmn') c')
+    as R2.
+  destruct R2; try solve [inversion Hinscope2].
+  remember (inscope_of_tmn F
+             (block_intro l1 ps1 (cs1' ++ nil)(insn_return rid RetTy Result))
+             (insn_return rid RetTy Result)) as R1. 
+  destruct R1; try solve [inversion Hinscope1].
+  split; auto.
+  split; auto.
+  SCase "1".
+    split; auto.
+    split; auto.  
+    split; auto. 
+    split. 
+    SSCase "1.1".
+      destruct cs'; simpl_env in *.
+      clear - HeqR2 Hinscope2 H1 H.
+      SSSCase "1.1.1".
+        apply inscope_of_cmd_tmn in HeqR2.
+        destruct HeqR2 as [ids2 [J1 J2]].        
+        rewrite <- J1.
+        remember (getCmdID' c') as R.
+        destruct c'; try solve [inversion H].
+        unfold returnUpdateLocals in H1. simpl in H1.
+        destruct R.
+          destruct n; inv HeqR.
+          remember (getOperandValue (los,nts) Mem' Result lc gl) as R1.
+          destruct R1; inv H1.
+          eapply wf_defs_updateAddAL; eauto.
+
+          destruct n; inv HeqR. inv H1.
+          eapply wf_defs_eq; eauto. 
+        
+      SSSCase "1.1.2".
+        apply inscope_of_cmd_cmd in HeqR2.
+        destruct HeqR2 as [ids2 [J1 J2]].        
+        rewrite <- J1.
+        remember (getCmdID' c') as R.
+        destruct c'; try solve [inversion H].
+        unfold returnUpdateLocals in H1. simpl in H1.
+        destruct R.
+          destruct n; inv HeqR.
+          remember (getOperandValue (los,nts) Mem' Result lc gl) as R1.
+          destruct R1; inv H1.
+          eapply wf_defs_updateAddAL; eauto.
+
+          destruct n; inv HeqR. inv H1.
+          eapply wf_defs_eq; eauto. 
+    SSCase "1.2".
+      exists l2. exists ps2. exists (cs2'++[c']).   
+      simpl_env. auto.
+Unfocus.
+
+Focus.
+Case "dsReturnVoid".
+  destruct HwfS1 as 
+    [HwfSystem [HmInS [
+     [HBinF1 [HFinPs1 [Hinscope1 [l1 [ps1 [cs1' Heq1]]]]]] 
+     [
+       [
+         [HBinF2 [HFinPs2 [Hinscope2 [l2 [ps2 [cs2' Heq2]]]]]] 
+         [HwfEC HwfCall]
+       ]
+       HwfCall'
+     ]
+    ]]]; subst.
+  remember (inscope_of_cmd F' (block_intro l2 ps2 (cs2' ++ c' :: cs') tmn') c')
+    as R2.
+  destruct R2; try solve [inversion Hinscope2].
+  remember (inscope_of_tmn F
+             (block_intro l1 ps1 (cs1' ++ nil)(insn_return_void rid))
+             (insn_return_void rid)) as R1. 
+  destruct R1; try solve [inversion Hinscope1].
+  split; auto.
+  split; auto.
+  SCase "1".
+    split; auto.
+    split; auto.
+    split; auto.
+    split.   
+    SSCase "1.1".
+      destruct cs'; simpl_env in *.
+      clear - HeqR2 Hinscope2 H HwfCall'.
+      SSSCase "1.1.1".
+        apply inscope_of_cmd_tmn in HeqR2.
+        destruct HeqR2 as [ids2 [J1 J2]].        
+        rewrite <- J1.
+        remember (getCmdID' c') as R.
+        destruct c'; try solve [inversion H].
+        destruct n; inversion HwfCall'.
+        simpl in HeqR. subst R.
+        eapply wf_defs_eq; eauto. 
+        
+      SSSCase "1.1.2".
+        apply inscope_of_cmd_cmd in HeqR2.
+        destruct HeqR2 as [ids2 [J1 J2]].        
+        rewrite <- J1.
+        remember (getCmdID' c') as R.
+        destruct c'; try solve [inversion H].
+        destruct n; inversion HwfCall'.
+        simpl in HeqR. subst R.
+        eapply wf_defs_eq; eauto. 
+
+    SSCase "1.2".
+      exists l2. exists ps2. exists (cs2'++[c']).   
+      simpl_env. auto.
+Unfocus.
+
+Focus.
+Case "dsBranch".
+  destruct HwfS1 as 
+    [HwfSystem [HmInS [
+     [HBinF1 [HFinPs1 [Hinscope1 [l3 [ps3 [cs3' Heq1]]]]]] 
+     [HwfEC _]]]
+    ]; subst.
+  remember (inscope_of_tmn F
+             (block_intro l3 ps3 (cs3' ++ nil)(insn_br bid Cond l1 l2))
+             (insn_br bid Cond l1 l2)) as R1. 
+  destruct R1; try solve [inversion Hinscope1].
+  split; auto.
+  split; auto.
+  split; auto.
+  SCase "1".
+    split. 
+      clear - H0. admit. (* static *)
+    split; auto.
+    split.
+      clear - H0 HeqR1 H1 Hinscope1 H.
+      eapply inscope_of_tmn_br in HeqR1; eauto.
+      destruct HeqR1 as [ids0' HeqR1].
+      destruct cs'.
+        destruct HeqR1 as [HeqR11 HeqR12]. 
+        rewrite <- HeqR11.
+        eapply wf_defs_br; eauto.
+
+        destruct HeqR1 as [HeqR11 HeqR12]. 
+        rewrite <- HeqR11.
+        eapply wf_defs_br; eauto.
+
+      exists l'. exists ps'. exists nil. simpl_env. auto.
+  split; auto.
+    admit. (* need a stronger wf_call that considers rets at all blocks *)    
+Unfocus.
+
+Focus.
+Case "dsBranch_uncond".
+  destruct HwfS1 as 
+    [HwfSystem [HmInS [
+     [HBinF1 [HFinPs1 [Hinscope1 [l3 [ps3 [cs3' Heq1]]]]]] 
+     [HwfEC _]]]
+    ]; subst.
+  remember (inscope_of_tmn F
+             (block_intro l3 ps3 (cs3' ++ nil)(insn_br_uncond bid l0))
+             (insn_br_uncond bid l0)) as R1. 
+  destruct R1; try solve [inversion Hinscope1].
+  split; auto.
+  split; auto.
+  split; auto.
+  SCase "1".
+    split. clear - H0. admit. (* static *)
+    split; auto.
+    split.
+      clear - H0 HeqR1 Hinscope1 H.
+      eapply inscope_of_tmn_br_uncond with (cs':=cs')(l':=l')(ps':=ps')
+        (tmn':=tmn') in HeqR1; eauto.
+      destruct HeqR1 as [ids0' HeqR1].
+      destruct cs'.
+        destruct HeqR1 as [HeqR11 HeqR12]. 
+        rewrite <- HeqR11.
+        eapply wf_defs_br_uncond; eauto.
+
+        destruct HeqR1 as [HeqR11 HeqR12]. 
+        rewrite <- HeqR11.
+        eapply wf_defs_br_uncond; eauto.
+
+      exists l'. exists ps'. exists nil. simpl_env. auto.
+  split; auto.
+    admit. (* need a stronger wf_call that considers rets at all blocks *)    
+Unfocus.
+
+Focus.
+Case "dsBop".
+  destruct HwfS1 as 
+    [HwfSystem [HmInS [
+     [HBinF1 [HFinPs1 [Hinscope1 [l3 [ps3 [cs3' Heq1]]]]]]
+     [HwfEC HwfCall]]]
+    ]; subst.
+  remember (inscope_of_cmd F
+             (block_intro l3 ps3 (cs3' ++ insn_bop id0 bop0 sz0 v1 v2 :: cs) tmn)
+             (insn_bop id0 bop0 sz0 v1 v2)) as R1. 
+  destruct R1; try solve [inversion Hinscope1].
+  split; auto.
+  split; auto.
+  split.
+  SCase "1".
+    split; auto.
+    split; auto.
+    split.  
+    SSCase "1.1".
+      destruct cs; simpl_env in *.
+      clear - HeqR1 Hinscope1 H.
+      SSSCase "1.1.1".
+        apply inscope_of_cmd_tmn in HeqR1.
+        destruct HeqR1 as [ids2 [J1 J2]].        
+        rewrite <- J1.
+        apply BOP_inversion in H.
+        admit. (* need to prove that gv3 is wf-typed. *)
+        
+      SSSCase "1.1.2".
+        apply inscope_of_cmd_cmd in HeqR1.
+        destruct HeqR1 as [ids2 [J1 J2]].        
+        rewrite <- J1.
+        admit. (* need to prove that gv3 is wf-typed. *)
+
+    SSCase "1.2".
+      exists l3. exists ps3. exists (cs3'++[insn_bop id0 bop0 sz0 v1 v2]).   
+      simpl_env. auto.
+  split; auto.
+Unfocus.
+
+Case "dsFBop". admit.
+Case "dsExtractValue". admit.
+Case "dsInsertValue". admit.
+Case "dsMalloc". admit.
+Case "dsFree". admit.
+Case "dsAlloca". admit.
+Case "dsLoad". admit.
+Case "dsStore". admit.
+Case "dsGEP". admit.
+Case "dsTrunc". admit.
+Case "dsExt". admit.
+Case "dsCast". admit.
+Case "dsIcmp". admit.
+Case "dsFcmp". admit.
+Case "dsSelect". admit.
+
+Focus.
+Case "dsCall".
+  destruct HwfS1 as [HwfSys [HmInS [HwfEC [HwfECs HwfCall]]]].
+  split; auto.
+  split; auto.
+  split.
+  SCase "1".
+    split. admit. (* static *)
+    split. admit. (* static *)
+    split.  
+      admit. (* need to prove that initial state is good! *)
+    exists l'. exists ps'. exists nil. simpl_env. auto.
+  split.
+  SCase "2".
+    split; auto.
+  SCase "3".
+    simpl.  
+    destruct tmn'; auto.
+      admit. (* static: void cannot be assigned as a call ret. *)
+Unfocus.
+
+Case "dsExCall". admit.
+Qed.
+
+Lemma state_tmn_typing : forall ifs s m f b tmn1 defs id1 lc,
+  wf_insn ifs s m f b (insn_terminator tmn1) ->
+  Some defs = inscope_of_tmn f b tmn1 ->
+  wf_defs f lc (AtomSetImpl.elements defs) ->
+  In id1 (getInsnOperands (insn_terminator tmn1)) ->
+  exists t, exists gv, lookupAL _ lc id1 = Some gv /\ wf_genericvalue gv t.
+Proof.
+  intros ifs s m f b tmn1 defs id1 lc HwfInstr Hinscope HwfDefs HinOps.
+  inv HwfInstr.
+Case "ret".
+  unfold getInsnOperands, getTerminatorOperands, getValueIDs in HinOps.
+  destruct value5 as [vid | vc]; try solve [inversion HinOps].
+  simpl in HinOps. 
+  destruct HinOps as [HinOps | HinOps]; try solve [inversion HinOps].
+  subst.
+  inv H7.
+  simpl in H6. unfold getValueIDs in H6. simpl in H6.
+  destruct id_list; inv H6.
+  simpl in H8.
+  inv H8. clear H16. 
+  inv H7.             
+  assert (isBindingInsn (lookupBindingViaIDFromFdef f i0) = ret insn') as J.
+    admit.
+  assert (J':=J).
+  apply H15 in J'. clear H15.
+  inv J'.
+  clear H8.
+  unfold isPhiNode in H11.
+  simpl in H11.
+  assert (notT (false = true)) as J'. 
+    intro J2. inversion J2.
+  apply H11 in J'. clear H11.
+  clear - J J' HwfDefs Hinscope H0.
+  assert (i0 `in` defs) as J1.
+    admit.
+  admit.
+Admitted.
+
+Lemma state_cmd_typing : forall ifs s m f b c defs id1 lc,
+  wf_insn ifs s m f b (insn_cmd c) ->
+  Some defs = inscope_of_cmd f b c ->
+  wf_defs f lc (AtomSetImpl.elements defs) ->
+  In id1 (getInsnOperands (insn_cmd c)) ->
+  exists t, exists gv, lookupAL _ lc id1 = Some gv /\ wf_genericvalue gv t.
+Admitted.
+
+
+Lemma wf_system__blockInFdefB__wf_block : forall b f ps los nts s ifs,
+  blockInFdefB b f = true -> 
+  InProductsB (product_fdef f) ps = true ->
+  moduleInSystemB (module_intro los nts ps) s = true ->
+  wf_system ifs s ->
+  wf_block ifs s (module_intro los nts ps) f b.
+Admitted.
+
+Lemma wf_system__lookup__wf_block : forall b f l0 ps los nts s ifs,
+  Some b = lookupBlockViaLabelFromFdef f l0 ->
+  InProductsB (product_fdef f) ps = true ->
+  moduleInSystemB (module_intro los nts ps) s = true ->
+  wf_system ifs s ->
+  wf_block ifs s (module_intro los nts ps) f b.
+Admitted.
+
+Lemma progress : forall S1,
+  wf_State S1 -> 
+    ds_isFinialState S1 = true \/ exists S2, exists tr, dsInsn S1 S2 tr.
+Proof.
+  intros S1 HwfS1.
+  destruct S1 as [s [los nts] ps ecs gl fs M].
+  destruct HwfS1 as [HwfSys1 [HmInS1 HwfECs]].
+  destruct ecs.
+    admit. (* we should rule out this case. *)
+
+  destruct e as [f b cs tmn lc als].
+  destruct HwfECs as [[HbInF [HfInPs [Hinscope [l1 [ps1 [cs1 Heq]]]]]] 
+                      [HwfECs HwfCall]].
+  subst b.
+  destruct cs.
+  Case "cs=nil".
+    remember (inscope_of_tmn f (block_intro l1 ps1 (cs1 ++ nil) tmn) tmn) as R.
+    destruct R; try solve [inversion Hinscope].
+    destruct tmn.
+    SCase "tmn=ret".
+      simpl in HwfCall.
+      destruct ecs.
+        simpl; auto.      
+
+        right.
+        destruct e as [f' b' cs' tmn' lc' als'].
+        destruct cs'; try solve [inversion HwfCall].
+        destruct c; try solve [inversion HwfCall]. clear HwfCall.
+        assert (exists M', free_allocas (los,nts) M als = Some M') as J.
+          admit.
+        destruct J as [M' J].
+        assert (exists lc'', 
+          returnUpdateLocals (los,nts) M' (insn_call i1 n t1 t2 v0 p) v lc lc' gl
+            = Some lc'') as Hretup.
+          unfold returnUpdateLocals. simpl.
+          destruct n.
+            exists lc'. auto.
+            
+            destruct v as [vid | vc].
+              assert (HwfInstr:=HbInF).
+              eapply wf_system__wf_insn in HwfInstr; eauto.
+              assert (exists t, exists gv, lookupAL _ lc vid = Some gv /\ 
+                wf_genericvalue gv t) as Hlkup.
+                assert (In vid (getInsnOperands (insn_terminator 
+                  (insn_return i0 t0 (value_id vid))))) as HinOps.
+                  simpl. auto.
+                eapply state_tmn_typing in HwfInstr; eauto.
+
+              destruct Hlkup as [gt [gv [Hlkup Hwfgv]]].
+              simpl.
+              rewrite Hlkup. exists (updateAddAL GenericValue lc' i1 gv). auto.
+
+              admit. (* what if a constant is stuck~? if int2ptr is not allowed,
+                        we should prove this, because globals are not changed!
+                      *)
+          
+            destruct Hretup as [lc'' Hretup].
+            exists (mkState s (los, nts) ps ((mkEC f' b' cs' tmn' lc'' als')::
+              ecs) gl fs M').
+            exists trace_nil.
+            eauto.  
+
+    SCase "tmn=ret void". admit.
+    SCase "tmn=br". admit.
+    SCase "tmn=br_uncond". 
+      right.
+      assert (exists B0, Some B0 = lookupBlockViaLabelFromFdef f l0) as HlkB.
+        admit. (* wf *)
+      destruct HlkB as [B0 HlkB].
+      destruct B0 as [l' ps' cs' tmn'].
+      assert (exists RVs, 
+        getIncomingValuesForBlockFromPHINodes (los, nts) M ps'
+          (block_intro l1 ps1 (cs1 ++ nil) (insn_br_uncond i0 l0)) gl lc =
+        Some RVs) as J.
+
+        eapply wf_system__blockInFdefB__wf_block in HbInF; eauto.
+        eapply wf_system__lookup__wf_block in HlkB; eauto.
+        clear - HeqR Hinscope HbInF HlkB.
+        inv HlkB. clear H9 H10 H7.
+        induction ps'; simpl.
+          exists nil. auto.
+
+          destruct a.
+          assert (exists v, getValueViaLabelFromValuels l2 l1 = Some v) as J.
+            admit. (*wf*)
+          destruct J as [v J].
+          rewrite J.
+          destruct v as [vid | vc].
+            inv H8.
+            assert (exists gv1, lookupAL GenericValue lc vid = Some gv1) as J1.
+              inv H6.              
+              inv H23.
+              admit.
+            destruct J1 as [gv1 J1].
+            rewrite J1. 
+            apply IHps' in H7.
+            destruct H7 as [RVs H7].
+            rewrite H7. 
+            exists ((i1, gv1) :: RVs). auto.
+
+            admit. (* constant *)
+      destruct J as [RVs J].
+      assert (exists lc', switchToNewBasicBlock (los, nts) M
+        (block_intro l' ps' cs' tmn') 
+        (block_intro l1 ps1 (cs1 ++ nil) (insn_br_uncond i0 l0)) gl lc = 
+          Some lc') as Hswitch.
+        unfold switchToNewBasicBlock. simpl.
+        rewrite J. 
+        exists (updateValuesForNewBlock RVs lc). auto.
+     destruct Hswitch as [lc' Hswitch].
+     exists (mkState s (los, nts) ps 
+              ((mkEC f (block_intro l' ps' cs' tmn') cs' tmn' lc' als)
+              ::ecs) gl fs M).
+     exists trace_nil. eauto.
+    SCase "tmn=unreachable". admit.
+
+  Case "cs<>nil".
+    admit.
+Qed.
 
 (*****************************)
 (*
